Second structural lemma, termination metric, proof for wilds case
Structural result for wilds
Define termination metric
Prove that wilds is smaller (including with simplification)
Refactor compile to include n and proof that it is large enough
More proof obligations - prove that bound we need is smaller in inductive cases
Remove some old code but still need to clean up more

proofs/core/Pattern.v
@@ -61,7 +61,7 @@ Equations dispatch (x: list pattern * A)
   (y:  (amap funsym (list (list pattern * A))) * list (list pattern * A) ) : 
   (amap funsym (list (list pattern * A))) * list (list pattern * A) 
   by wf (pat_list_size (fst x)) lt  :=
-  dispatch (nil, _) y := (*impossible*) (amap_empty, nil);
+  dispatch (nil, _) y := (*impossible*) y;
   dispatch (Pvar x :: pl, a) (cases, wilds) := 
     let a := mk_let x t a in
     (union_cases pl a types cases, (pl, a) :: wilds);
@@ -96,7 +96,7 @@ Definition simplify_single (x: list pattern * A) : list (list pattern * A) :=
     let (ps, a) := x in
     match ps with
     | p :: ptl => 
-      map (fun '(p1, y) => (p1 :: ptl, y)) (simplify_aux a p)
+      map (fun x => (fst x :: ptl, snd x)) (simplify_aux a p)
     | nil => nil
     end.
 
@@ -126,34 +126,29 @@ Definition dispatch2 (rl: list (list pattern * A)) :=
   dispatch2_gen (simplify rl).
 
 (*We need this for the odd induction principle*)
-Lemma dispatch_equiv_aux x base 
-  (Hnull: negb (null (fst x))):
+Lemma dispatch_equiv_aux x base :
   dispatch x base =
   fold_right dispatch2_aux base (simplify_single x).
 Proof.
-  revert x base Hnull.
-  apply (dispatch_elim (fun x base rec => negb (null (fst x)) -> 
-    rec = fold_right dispatch2_aux base (simplify_single x))); auto.
-  - intros. discriminate.
-  - intros p q pl a cases wilds IH1 IH2. simpl in *.
-    intros _.
-    rewrite map_app, fold_right_app.
-    rewrite <- IH1; auto.
+  apply dispatch_elim; auto.
+  intros p q pl a cases wilds IH1 IH2. simpl in *.
+  rewrite map_app, fold_right_app.
+  rewrite <- IH1; auto.
 Qed.
  
 (*Now we prove equivalence*)
-Lemma dispatch_equiv rl (Hrl: Forall (fun x => negb (null (fst x))) rl):
+Lemma dispatch_equiv rl:
   dispatch1 rl = dispatch2 rl.
 Proof.
   unfold dispatch2, dispatch2_gen, dispatch1.
   induction rl as [|[pl a] ps IH]; simpl; auto.
-  inversion Hrl as [|? ? Hpl Hps]; subst; simpl in *.
   unfold simplify in *. simpl.
   rewrite fold_right_app.
   destruct pl as [| phd ptl]; simpl in *; try discriminate.
-  rewrite <- IH; auto.
-  destruct (fold_right dispatch (amap_empty, []) ps) as [cases1 wilds1] eqn : Hd2.
-  apply dispatch_equiv_aux. reflexivity.
+  - rewrite dispatch_equation_1. auto. 
+  - rewrite <- IH; auto. 
+    destruct (fold_right dispatch (amap_empty, []) ps) as [cases1 wilds1] eqn : Hd2; auto.
+    apply dispatch_equiv_aux.
 Qed.
 End Dispatch.
 
@@ -188,22 +183,33 @@ Definition term_list_size (l: list term) : nat :=
 
 (*None = NonExhaustive*)
 
-Definition compile_size (l: list (list pattern * A)) : nat :=
-  sum (map pat_list_size (map fst l)).
+(* Definition compile_size (l: list (list pattern * A)) : nat :=
+  sum (map pat_list_size (map fst l)). *)
+
+(*TODO: move*)
+Search "bind".
+Definition option_bind {A B: Type} (o: option A) (f: A -> option B) : option B :=
+  match o with
+  | Some x => f x
+  | None => None
+  end.
 
 Section Populate.
 Variable (is_constr : funsym -> bool).
-Fixpoint populate  (acc : amap funsym (list pattern) * list (funsym * list vty * list pattern)) 
-        (p: pattern) : amap funsym (list pattern) * list (funsym * list vty * list pattern) :=
+(*NOTE: populate will give option - want to ensure everything in pattern is constructor*)
+Fixpoint populate  (acc : option (amap funsym (list pattern) * list (funsym * list vty * list pattern))) 
+        (p: pattern) : option (amap funsym (list pattern) * list (funsym * list vty * list pattern)) :=
         match p with
         | Pwild => acc
         | Pvar _ => acc
         | Pconstr fs params ps =>
-          let (css, csl) := acc in
+          option_bind acc
+          (fun acc => 
+            let (css, csl) := acc in
             if is_constr fs then
-            if amap_mem funsym_eq_dec fs css then acc else
-            (amap_set funsym_eq_dec css fs ps, (fs, params, ps) :: csl)
-          else acc (*impossible case - Why3 throws exception here*)
+              if amap_mem funsym_eq_dec fs css then Some acc else
+              Some (amap_set funsym_eq_dec css fs ps, (fs, params, ps) :: csl)
+            else None (*exception - impossible by typing*))
         | Por p1 p2 => populate (populate acc p1) p2
         | Pbind p _ => populate acc p
         end.
@@ -230,7 +236,7 @@ Definition filter_map {A B: Type} (f: A -> option B) (l: list A): list B :=
 Check amap_get.
 
 Definition populate_all (is_constr: funsym -> bool) (rl: list (list pattern * A)) :=
-  fold_left (populate is_constr) (map (fun x => List.hd Pwild (fst x)) rl) (amap_empty, nil).
+  fold_left (populate is_constr) (map (fun x => List.hd Pwild (fst x)) rl) (Some (amap_empty, nil)).
 Check populate_all.
 
 Definition pat_at_head (p: pattern) (r: list pattern * A) : bool :=
@@ -548,372 +554,278 @@ Proof.
       rewrite Hd in Hnone; apply Hnone. auto.
 Qed.
 
-(*START: do default structural lemma*)
+(*Second main structural lemma: the matrix D*)
+Print dispatch2_aux.
 
-
+Lemma dispatch2_gen_snd (types: amap funsym (list pattern)) rl:
+  snd (dispatch2_gen types rl) = filter_map (fun x =>
+    match (fst x) with
+    | Pwild :: ps => Some (ps, snd x)
+    | _ => None
+    end ) rl.
+Proof.
+  induction rl as [| [pl a] rtl IH]; simpl; auto.
+  unfold dispatch2_aux; simpl.
+  destruct (dispatch2_gen types rtl ) as [cases wilds]; simpl in *.
+  destruct pl as [| p ps]; auto.
+  destruct p; auto; simpl.
+  f_equal; auto.
+Qed.
 
 (*Termination Metric*)
 
+(*The termination metric is complicated. The compile function is not structurally recursive.
+  The natural choice for the termination metric is the sum of the sizes of the patterns in the input list,
+  since for a constructor c(ps) :: pl, it becomes ps :: pl, decreasing the size.
+  However, this does not work: the size gets bigger when we simplify to remove "or" patterns.
+  An alternative is then to make the metric the sum of the products of 2^(size p) for each p in each list.
+  This ensures that Por p q :: pl is bigger than p :: pl + q :: pl
+  But this also doesn't work: when we add the extra (length (s_args c)) Pwilds in the matrix S, we end up
+  with a bigger matrix.
+  A solution is a compbined metric: we add the size of a Pwild, but multiply the others.
+  Then we make the Pconstr part big enough to compensate for the (bounded) sum of Pwilds that we add.
+  TODO: make sure this works*)
+
+(*A more complicated pattern size metric*)
+
+
+Definition pat_size_op (f: pattern -> nat) (p1 p2: pattern) : nat :=
+  match p1 with
+  | Pwild => f p1 + f p2
+  | _ => (*TODO: is mult enough or do we need 2^(size p)?*)
+      2 ^ (f p1) * 2 ^ (f p2)
+  end.
+
+Definition pat_iter_op (f: pattern -> nat) :=
+  fix pat_iter_op (l: list pattern) : nat :=
+    match l with
+    | nil => 1
+    (*| [Pwild] => 2*) (*does NOT work - then does not decrease*)
+    | Pwild :: tl => 1 + pat_iter_op tl
+    | p :: tl => 2 ^ (f p) * (pat_iter_op tl)
+    end.
+
+Fixpoint pat_size_mixed (n: nat) (p: pattern) : nat :=
+  match p with
+  | Pwild => 1
+  | Pvar _ => 1
+  | Pbind p x => 1 + pat_size_mixed n p
+  | Por p1 p2 => 1 + pat_size_mixed n p1 + pat_size_mixed n p2 (*TODO?*)
+  | Pconstr c _ ps => 1 + n + pat_iter_op (pat_size_mixed n) ps
+  end.
+
+Definition pat_list_size_mixed (n: nat) (l: list pattern) : nat :=
+  pat_iter_op (pat_size_mixed n) l.
+
+(*And the metrix*)
+Definition compile_size (n: nat) (l: list (list pattern * A)) : nat :=
+  sum (map (fun x => pat_list_size_mixed n (fst x)) l).
+
+(*TODO: move*)
+Lemma sum_app l1 l2:
+  sum (l1 ++ l2) = sum l1 + sum l2.
+Proof.
+  induction l1; simpl; auto. lia.
+Qed.
+
+Lemma compile_size_app n l1 l2:
+  compile_size n (l1 ++ l2) = compile_size n l1 + compile_size n l2.
+Proof.
+  unfold compile_size. rewrite map_app.
+  apply sum_app.
+Qed.
+
+Lemma compile_size_cons n a l:
+  compile_size n (a :: l) = pat_list_size_mixed n (fst a) + compile_size n l.
+Proof. reflexivity. Qed.
+  
+
 (*Termination Proofs*)
+(*compile_size (compile_size_bound (snd (dispatch1 t types rl))) (snd (dispatch1 t types rl)) <
+compile_size (compile_size_bound (phd :: ptl)) (phd :: ptl)*)
+(*Think we will need: take n larger than compile_size_bound (so that n does not change recursively,
+  for IH, easy*)
+
+Lemma add_lt_pow n m:
+  1 <= m ->
+  1 <= n ->
+  S n <= 2 ^ m * n.
+Proof.
+  intros Hm Hn.
+  induction m; try lia.
+  destruct m.
+  - simpl. lia.
+  - rewrite Nat.pow_succ_r'. nia.
+Qed.
+
+Lemma pat_size_mixed_geq_1 n p:
+  1 <= pat_size_mixed n p.
+Proof.
+  induction p; simpl; lia.
+Qed.
+
+Lemma mul_geq_1 n m:
+  1 <= m ->
+  1 <= n ->
+  1 <= (m * n).
+Proof.
+nia.
+Qed.
+
+Lemma pow_geq_1 n m:
+  1 <= n ->
+  1 <= n ^ m.
+Proof.
+  induction m; simpl; intros; lia.
+Qed.
+
+Lemma pat_list_size_mixed_geq n ps:
+  1 <= pat_list_size_mixed n ps.
+Proof.
+  induction ps; simpl; try lia.
+  destruct a; try solve[simpl; lia].
+  - simpl. apply mul_geq_1; auto.
+    eapply Nat.le_trans. 2: apply Nat.le_add_r.
+    apply pow_geq_1. lia.
+  - apply mul_geq_1; auto. apply pow_geq_1. lia.
+  - apply mul_geq_1; auto. apply pow_geq_1. lia.
+Qed.
+  
+(*We do NOT have equality: this is crucial for adding pwilds, but we do need that it is
+  sometimes a strict equality for the "or" case of simplifying*)
+Lemma pat_list_size_mixed_cons n p pl:
+  pat_list_size_mixed n (p :: pl) <= 2 ^ pat_size_mixed n p * pat_list_size_mixed n pl.
+Proof.
+  simpl. destruct p; auto. destruct pl.
+  - simpl; lia.
+  - set (y:=(pat_list_size_mixed n (p :: pl))). apply add_lt_pow; try lia.
+    + apply pat_size_mixed_geq_1.
+    + apply pat_list_size_mixed_geq.
+Qed.
+
+Lemma lt_le_0_1 n:
+  0 < n <-> 1 <= n.
+Proof. lia. Qed.
+ 
+Lemma dispatch_smaller n t types rhd rtl:
+  compile_size n (snd (dispatch t types rhd rtl)) < pat_list_size_mixed n (fst rhd) + compile_size n (snd rtl).
+Proof.
+  apply dispatch_elim; intros; auto; try solve[simpl; lia].
+  - simpl. rewrite compile_size_cons. simpl. 
+    pose proof (pat_list_size_mixed_geq n pl). lia.
+  - simpl. rewrite <- (Nat.add_0_l (compile_size n wilds)) at 1. apply Nat.add_lt_mono_r.
+    apply lt_le_0_1. apply mul_geq_1.
+    + eapply Nat.le_trans. 2: apply Nat.le_add_r. apply pow_geq_1. lia.
+    + apply pat_list_size_mixed_geq.
+  - simpl. eapply Nat.lt_le_trans. apply H0.
+    eapply Nat.le_trans. apply Nat.add_le_mono_l. apply Nat.lt_le_incl, H. 
+    simpl snd. rewrite !Nat.add_assoc. apply Nat.add_le_mono_r. simpl fst.
+    eapply Nat.le_trans. apply Nat.add_le_mono. apply pat_list_size_mixed_cons. apply pat_list_size_mixed_cons.
+    rewrite Nat.add_0_r, !Nat.pow_add_r, Nat.mul_add_distr_r.
+    apply Nat.add_le_mono.
+    + apply Nat.mul_le_mono_r. rewrite <- (Nat.mul_1_r (2 ^ (pat_size_mixed n p))) at 1.
+      apply Nat.mul_le_mono; auto. apply pow_geq_1; lia.
+    + apply Nat.mul_le_mono_r. rewrite <- (Nat.mul_1_l (2 ^ (pat_size_mixed n q))) at 1.
+      apply Nat.mul_le_mono; auto. apply pow_geq_1; lia.
+  - eapply Nat.le_trans. apply H. apply Nat.add_le_mono_r.
+    simpl fst. eapply Nat.le_trans. apply pat_list_size_mixed_cons.
+    simpl. nia.
+Qed.
+
+Lemma dispatch1_smaller n t types rl:
+  compile_size n (snd (dispatch1 t types rl)) <= compile_size n rl.
+Proof.
+  induction rl as [| rhd rtl IH]; auto.
+  simpl. eapply Nat.le_trans. apply Nat.lt_le_incl, dispatch_smaller.
+  simpl. rewrite compile_size_cons. lia.
+Qed.
+
+(*Old, weaker lemma*)
+(*
+Lemma dispatch_smaller n t types rhd rtl:
+  compile_size n (snd (dispatch t types rhd rtl)) <= pat_list_size_mixed n (fst rhd) + compile_size n (snd rtl).
+Proof.
+  apply dispatch_elim; intros; auto; try solve[simpl; lia].
+  - simpl. rewrite compile_size_cons. simpl. lia.
+  - simpl. rewrite compile_size_cons. simpl. destruct pl; simpl; lia.
+  - simpl. eapply Nat.le_trans. apply H0.
+    eapply Nat.le_trans. apply Nat.add_le_mono_l. apply H.
+    simpl snd. rewrite !Nat.add_assoc. apply Nat.add_le_mono_r. simpl fst.
+    eapply Nat.le_trans. apply Nat.add_le_mono. apply pat_list_size_mixed_cons. apply pat_list_size_mixed_cons.
+    rewrite Nat.add_0_r, !Nat.pow_add_r, Nat.mul_add_distr_r.
+    apply Nat.add_le_mono.
+    + apply Nat.mul_le_mono_r. rewrite <- (Nat.mul_1_r (2 ^ (pat_size_mixed n p))) at 1.
+      apply Nat.mul_le_mono; auto. apply pow_geq_1; lia.
+    + apply Nat.mul_le_mono_r. rewrite <- (Nat.mul_1_l (2 ^ (pat_size_mixed n q))) at 1.
+      apply Nat.mul_le_mono; auto. apply pow_geq_1; lia.
+  - eapply Nat.le_trans. apply H. apply Nat.add_le_mono_r.
+    simpl fst. eapply Nat.le_trans. apply pat_list_size_mixed_cons.
+    simpl. nia.
+Qed.*)
+
+
 
 (*TODO: do we need to know that only Pwild/Pconstr*)
 
 (*First, let's prove something about [types] and [cslist] - should be easier*)
 (*Probably need map equivalence*)
 
-
-
-(*Lemma dispatch2_gen_fst (types: amap funsym (list pattern)) rl cs args
-  (*Cannot be iff for IH*)
-  (*(Htypes: forall cs args, amap_get funsym_eq_dec types cs = Some args ->
-    exists ps tys a, In (Pconstr cs tys args :: ps, a) rl)*):
-  amap_get funsym_eq_dec types cs = Some args ->
-  amap_get funsym_eq_dec (fst (dispatch2_gen types rl)) cs = Some
-    (filter_map (fun x =>
-    let ps := fst x in
-    let a := snd x in
-    let p := hd Pwild ps in
-    let ps := tl ps in
-    match p with
-    | Pwild => Some (repeat Pwild (length args) ++ ps, a)
-    | Pconstr fs tys pats =>
-        if funsym_eqb fs cs then Some (rev pats ++ ps, a) else None
-    | _ => None
-    end) rl).
-Proof.
-  intros Htypesget.
-  induction rl as [| [ps a] rtl IH]; simpl.
-  - apply Htypes in Htypesget. destruct_all; contradiction.
-  - simpl in Htypes. rewrite amap_empty_get. in Hget. discriminate.
-  - destruct (dispatch2_gen types rtl) as [cases wilds] eqn : Hrec.
-    simpl in *. 
-
-
-  (*(rl_wf: forall c tys1 tys2 ps1 ps2 l1 l2, In (Pconstr c tys1 ps1) (concat (map fst l1)) -> 
-    In (Pconstr c tys2 ps2) (concat (map fst l2)) -> length tys1 = length tys2 /\ length ps1 = length ps2):*):
-  amap_get funsym_eq_dec (fst (dispatch2_gen types rl)) cs = Some l ->
-  l = filter_map (fun x =>
-    let ps := fst x in
-    let a := snd x in
-    let p := hd Pwild ps in
-    let ps := tl ps in
-    match (amap_get funsym_eq_dec types cs) with
-    | None => (*impossible*) None
-    | Some args =>
-        match p with
-        | Pwild => Some (repeat Pwild (length args) ++ ps, a)
-        | Pconstr fs tys pats =>
-            if funsym_eqb fs cs then Some (rev pats ++ ps, a) else None
-        | _ => None
-        end 
-    end) rl.
-Proof.
-
-
-Lemma dispatch2_gen_fst (types: amap funsym (list pattern)) rl cs l
-
-
-  (*(rl_wf: forall c tys1 tys2 ps1 ps2 l1 l2, In (Pconstr c tys1 ps1) (concat (map fst l1)) -> 
-    In (Pconstr c tys2 ps2) (concat (map fst l2)) -> length tys1 = length tys2 /\ length ps1 = length ps2):*):
-  amap_get funsym_eq_dec (fst (dispatch2_gen types rl)) cs = Some l ->
-  l = filter_map (fun x =>
-    let ps := fst x in
-    let a := snd x in
-    let p := hd Pwild ps in
-    let ps := tl ps in
-    match (amap_get funsym_eq_dec types cs) with
-    | None => (*impossible*) None
-    | Some args =>
-        match p with
-        | Pwild => Some (repeat Pwild (length args) ++ ps, a)
-        | Pconstr fs tys pats =>
-            if funsym_eqb fs cs then Some (rev pats ++ ps, a) else None
-        | _ => None
-        end 
-    end) rl.
-Proof.
-  induction rl as [| [ps a] rtl IH]; simpl.
-  - intros Hget. rewrite amap_empty_get in Hget. discriminate.
-  - destruct (dispatch2_gen types rtl) as [cases wilds] eqn : Hrec.
-    simpl in *. 
- discrimintae. Search amap_empty.
-
-Proof.
-  
-
-
-  
-  l = map (filter (fun x =>
-    let ps := fst x in
-    let a := snd x in
-  rl).
-  *)
-Print compile_size.
-Lemma compile_size_cons p l:
-  compile_size (p :: l) = pat_list_size (fst p) + compile_size l.
-Proof.
-  reflexivity.
-Qed.
-
-Lemma compile_size_app l1 l2:
-  compile_size (l1 ++ l2) = compile_size l1 + compile_size l2.
-Proof.
-  induction l1; simpl; auto.
-  rewrite !compile_size_cons. lia.
-Qed.
-
-Lemma compile_size_concat l:
-  compile_size (concat l) = sum (map compile_size l).
-Proof.
-  induction l; simpl; auto.
-  rewrite compile_size_app. lia.
-Qed.
-
-Print simplify_single.
-Print simplify_aux.
-
-Lemma pat_list_size_nil: pat_list_size nil = 0.
-Proof. reflexivity. Qed.
-
-(*TODO: unify these*)
-Lemma pat_list_size_app l1 l2:
-  pat_list_size (l1 ++ l2) = pat_list_size l1 + pat_list_size l2.
-Proof.
-  induction l1; simpl; auto. rewrite !pat_list_size_cons. lia.
-Qed.
-
-Lemma simplify_aux_smaller t a p:
-  pat_list_size (map fst (simplify_aux t a p)) <= pat_size p.
-Proof.
-  revert a.
-  induction p; simpl; intros a; try reflexivity.
-  - rewrite pat_list_size_cons, pat_list_size_nil; simpl; lia.
-  - rewrite map_app, pat_list_size_app. specialize (IHp1 a); specialize (IHp2 a).  lia.
-  - specialize (IHp (mk_let v t a)). lia.
-Qed.
-
-(*The point is that even when we split, this is all a part of the original
-  However, the pattern can indeed get bigger
-  example (simple): (Pvar x | Pvar y) :: Pwild becomes (Pvar x :: Pwild), (Pvar y :: Pwild) - 
-    the size is clearly larger
-  maybe instead we want the maximum? but that doesn't work either
-  if we did maximum, let's see
-  but by the dispatch, it should work?*)
-Print dispatch1.
-
-Lemma compile_size_nil: compile_size nil = 0.
-Proof. reflexivity. Qed.
-
-(*Another compile measures*)
-Definition iter_mult (l: list nat) : nat :=
-  fold_right mult 1 l.
-Definition pattern_list_size' (ps: list pattern) : nat :=
-  iter_mult (map (fun p => 2 ^ (pat_size p)) ps).
-Check compile_size.
-Print compile_size.
-Definition compile_size' (l: list (list pattern * A)) : nat :=
-  sum (map pattern_list_size' (map fst l)).
-
-Lemma compile_size_cons' a l:
-  compile_size' (a :: l) = pattern_list_size' (fst a) + compile_size' l.
-Proof.
-  reflexivity. Qed.
-Lemma compile_size_nil': compile_size' nil = 0.
-Proof. reflexivity. Qed.
-
-Lemma pattern_list_size_cons' p l:
-  pattern_list_size' (p :: l) = 2 ^ (pat_size p) * (pattern_list_size' l).
-Proof. reflexivity. Qed.
-Search (( ?x + ?y) * ?z).
-Search (?x ^ (?y + ?z)).
-Search (?x + ?y <= ?w + ?v).
- Search (?x <= ?y * ?x).
-Search (?x <= ?y ^ ?z).
-
-Lemma pow_geq_1 n m:
-  n <> 0 ->
-  1 <= n ^ m.
-Proof.
-  induction m; simpl; lia.
-Qed.
-
-Lemma mul_le n m:
-  1 <= m ->
-  n <= m * n.
-Proof.
-pose proof (Arith_prebase.mult_O_le_stt n m). lia.
-Qed. 
-
-Lemma dispatch_smaller t types a rl:
-  compile_size' (snd (dispatch t types a rl)) <= compile_size' (a :: (snd rl)).
-Proof.
-  apply dispatch_elim; intros; simpl.
-  - rewrite compile_size_nil'; lia.
-  - rewrite !compile_size_cons'; simpl. rewrite pattern_list_size_cons'.
-    simpl. lia.
-  - rewrite compile_size_cons'; simpl. lia.
-  - rewrite !compile_size_cons'; simpl. 
-    rewrite pattern_list_size_cons'. simpl. lia.
-  - simpl in *. revert H H0. rewrite !compile_size_cons'; simpl.
-    rewrite !pattern_list_size_cons'; simpl. 
-    intros Hlt1 Hlt2. eapply Nat.le_trans. apply Hlt2.
-    apply (Nat.add_le_mono_l _ _ (2 ^ pat_size p * pattern_list_size' pl)) in Hlt1.
-    eapply Nat.le_trans. apply Hlt1. clear.
-    (*Why we needed exponents*)
-    rewrite Nat.add_0_r. rewrite !Nat.add_assoc. apply Nat.add_le_mono_r.
-    rewrite Nat.mul_add_distr_r, !Nat.pow_add_r.
-    apply Nat.add_le_mono.
-    + rewrite <- (Nat.mul_comm (2^ (pat_size q))). rewrite <- Nat.mul_assoc. apply mul_le, pow_geq_1. auto.
-    + rewrite <- Nat.mul_assoc. apply mul_le, pow_geq_1. auto.
-  - rewrite !compile_size_cons' in H |- *. simpl in *. rewrite pattern_list_size_cons' in H |- *; simpl in *.
-    eapply Nat.le_trans. apply H. rewrite Nat.add_0_r. nia.
-Qed.
-
-(*START: use this metric, prove the full result (maybe use simplify but prob not)*)
-      
-
-
- assert (1 <= pat_size q) by admit. nia. lia.
-    
-    
-    
-    Search "distr". 
-
- nia.
-
-    Search (?z + ?x <= ?z + ?y).
-    assert (Hlt3: 2 ^ pat_size p * pattern_list_size' pl +
-      
-2 ^ pat_size p * pattern_list_size' pl +
-
- nia.
-
-
-
- nia. lia.
-   lia.
-    nia.
-
- lia. 
-
- lia.
-
-Lemma dispatch_smaller t types a rl:
-  compile_size (snd (dispatch t types a rl)) <= compile_size (a :: (snd rl)).
-Proof.
-apply dispatch_elim.
-- intros. simpl. rewrite compile_size_nil; auto. lia.
-- intros. simpl. rewrite !compile_size_cons. simpl. unfold pat_list_size. lia.
-- intros. simpl. rewrite compile_size_cons. simpl. lia.
-- intros; simpl. rewrite !compile_size_cons. simpl. unfold pat_list_size; lia.
-- intros; simpl. rewrite !compile_size_cons; simpl in *.
-  rewrite !compile_size_cons in H, H0. simpl in *.
-  rewrite !pat_list_size_cons in H, H0; simpl in *.
-  (*Doesn't work: "or" becomes larger
-    So what is the termination metric? - maybe it is the 
-
-    is it possible to not terminate?
-
-    so if we have (p1 | p2) ; Pwild, end up with
-      (p1 :: Pwild), (p2 :: Pwild)
-
-    what if we do exponentially decreasing:
-    like sum (2 ^ size p) (or mult?)
-    2 ^ (|p1| + |p2| + 1) = 2 * 2^(|p1|) * 2 ^(|p2|)
-    which is larger than  2^(|p1|) * 2^(|p2|)
-
-    so this should work
-    and same for the terms
-
-    will be more complicated
-
-    like: 2^(length l) * 1 + ...
-    would be smaller if this is smaller
-    otherwise, Por = |p1| + |p2| + 1, so
-
-
- lia.
-
- lia.
-  
-
- lia. 
-
- rewrite compile_size_cons. simpl. rewrite compile_size_nil.
-Search dispatch.
-Admitted.
-
-
-Lemma dispath1_smaller t types rl:
-  compile_size (snd (dispatch1 t types rl)) <= compile_size rl.
-Proof.
-  induction rl; simpl; auto.
-
-
-  
-
-  Print dispatch1.
-
-Lemma simplify_single_smaller t ps a:
-  compile_size (simplify_single t (ps, a)) <= pat_list_size ps.
-Proof.
-  unfold simplify_single.
-  destruct ps; auto.
-  rewrite pat_list_size_cons.
-  assert (forall rl, compile_size (map (fun '(p1, y) => (p1 :: ps, y)) rl) =
-    pat_list_size (map fst rl) + pat_list_size ps).
-  {
-    intros rl. induction rl; simpl.
-
-
-  Print simplify_single.
-  revert a.
-  induction ps as [|phd ptl IH]; intros a; simpl; auto.
-  rewrite pat_list_size_cons.
-  destruct phd; simpl.
-  - rewrite compile_size_cons; simpl. unfold compile_size; simpl.
-  Search pat_list_size.
-  Print simplify_single.
-
-Lemma simplify_smaller t rl : compile_size (simplify t rl) <= compile_size rl.
-Proof.
-  unfold simplify.
-  induction rl; simpl; try lia.
-  rewrite compile_size_app, compile_size_cons.
-  (*TODO: lemma?*)
-  assert (hhd: compile_size (simplify_single t a) <= pat_list_size (fst a)).
-  {
-    destruct a as [ps a]; simpl in *.
-    destruct ps as [| phd ptl]; simpl; auto.
-    
-    unfold simplify_aux.
-    simpl.
-
-
-  unfold simplify_single. destruct a as [ps a]; simpl in *.
-  destruct ps as 
-  Print simplify_single.
-  simpl.
-
-
-  rewrite compile_size_concat.
-  induction rl; simpl; try lia.
-  rewrite compile_
-
-Lemma wild_smaller t types rl: compile_size (snd (dispatch2 t types rl)) < compile_size rl.
-Proof.
-  unfold dispatch2. Check simplify t rl.
-
-
 (*Let's try this*)
 Definition dep_let (A: Type) (x: A) : {y: A | y = x} := exist _ x eq_refl.
 Obligation Tactic := idtac.
+
+(*The bound we give: (length rl) * (max size of s_args in rl)*)
+Definition get_constrs_in (rl: list (list pattern * A)) : list funsym :=
+  filter_map (fun y =>
+    match (fst y) with
+    | Pconstr f _ _ :: _ => Some f
+    | _ => None
+    end) rl.
+Definition iter_max (l: list nat) : nat :=
+  fold_right max 0 l.
+Definition compile_size_bound (rl: list (list pattern * A)) : nat :=
+  length (simplify tm_d rl) * (iter_max (map (fun (c: funsym) => length (s_args c)) (get_constrs_in rl))).
+
+Fixpoint split (l: list nat) : (list nat * list nat) :=
+  match l with
+  | nil => (nil, nil)
+  | [x] => ([x], nil)
+  | x :: y :: tl => let s := split tl in (x :: fst s, y :: snd s)
+  end.
+
+Definition pluslen (l1 l2: list nat) := length l1 + length l2.
+
+Equations merge (l1 l2: list nat) : list nat by wf (pluslen l1 l2) :=
+  merge (x1 :: t1) (x2 :: t2) => if Nat.leb x1 x2 then x1 :: merge t1 (x2 :: t2) else x2 :: merge (x1 :: t1) t2;
+  merge nil l1 => l1;
+  merge l2 nil => l2.
+Next Obligation.
+  intros. simpl. unfold pluslen; simpl. lia.
+Defined.
+Next Obligation.
+  intros. unfold pluslen; simpl. lia.
+Defined.
+
+Definition compile_size' (x: nat * list (list pattern * A)) : nat :=
+  compile_size (fst x) (snd x).
+Definition rl_wf (x: nat * list (list pattern * A)) : Prop :=
+  (fst x) >= compile_size_bound (snd x).
+
+(* Fixpoint merge (l1 l2: list nat) : list nat :=
+  match l1, l2 with
+  | x1 :: t1, x2 :: t2 => if x1 <= x2 then x1 :: merge t1 l2 else x2 :: merge l1 t2
+
+Equations mergesort (l1 l2: list nat) by wf (length l1 + length l2) : list nat :=
+   *)
+
+
 (*NOTE: will try to do with pattern, I think that is terminating*)
-Equations compile (tl: list (term * vty)) (rl: list (list pattern * A)) : option A 
-  by wf (compile_size rl) lt :=
-  compile _ [] := None;
-  compile [] ((_, a) :: _) => Some a;
-  compile ((t, ty) :: tl) rl =>
+(*TODO: why does equations not support function of multiple params?*)
+Equations compile (tl: list (term * vty)) (rl: nat * list (list pattern * A)) (Hrl: rl_wf rl)
+  : option A  by wf (compile_size' rl) lt :=
+  compile _ (n, []) Hn := None;
+  compile [] (n, (_, a) :: _) Hn => Some a;
+  compile ((t, ty) :: tl) (n, rl) Hn =>
     (*No bare*)
     (*extract the set of constructors*)
     let css :=
@@ -928,10 +840,12 @@ Equations compile (tl: list (term * vty)) (rl: list (list pattern * A)) : option
 
     (*Map every constructor ocurring at the head of the pattern list to the
       list of its args*)
-    let types_cslist :=
+    let types_cslist := populate_all is_constr rl in
+    match types_cslist as o return o = types_cslist -> _ with
+    | None => fun _ => None
+    | Some types_cslist => fun Htypes => 
       (*NOTE: we don't have maps, not ideal*)
-      fold_left (populate is_constr) (map (fun x => List.hd Pwild (fst x)) rl) (amap_empty, nil) 
-    in 
+      (* fold_left (populate is_constr) (map (fun x => List.hd Pwild (fst x)) rl) (amap_empty, nil)  *)
     let types := fst types_cslist in
     let cslist := snd types_cslist in
     
@@ -948,13 +862,13 @@ Equations compile (tl: list (term * vty)) (rl: list (list pattern * A)) : option
       end in
       compile (rev al ++ tl) l in*)
 
-    let comp_wilds (_: unit) := compile tl wilds in
+    let comp_wilds (_: unit) := compile tl (n, wilds) _ in
 
     (*TODO: default case here*)
     let comp_full (_: unit) :=
       let no_wilds := forallb (fun f => amap_mem funsym_eq_dec f types) css in
       let base : option (list (pattern * A)) := if no_wilds then Some nil else (*TODO: bind*)
-       match compile tl wilds with
+       match compile tl (n, wilds) _ with
         | None => None
         | Some x => Some [(Pwild, x)]
       end in
@@ -978,7 +892,7 @@ Equations compile (tl: list (term * vty)) (rl: list (list pattern * A)) : option
           | None => nil (*impossible*)
           | Some l => l
           end in
-          compile (rev al ++ tl) l in
+          compile (rev al ++ tl) (n, l) _ in
         match (comp_cases cs (combine al (map snd vl))) with
         | None => None
         | Some v => Some ((Pconstr cs params pl, v) :: acc)
@@ -1005,7 +919,7 @@ Equations compile (tl: list (term * vty)) (rl: list (list pattern * A)) : option
       | None => nil (*impossible*)
       | Some l => l
       end in
-      compile (rev al ++ tl) l in
+      compile (rev al ++ tl) (n, l) _ in
 
       if is_constr cs then
         if amap_mem funsym_eq_dec cs types then comp_cases cs (combine al
@@ -1013,8 +927,45 @@ Equations compile (tl: list (term * vty)) (rl: list (list pattern * A)) : option
       else comp_full tt
     | _ => 
       comp_full tt 
-    end.
+    end 
+end eq_refl.
 Next Obligation.
+intros t ty tl n phd ptl Hn compile rl css is_constr types_cslist t2 Heqt2 types cslist casewild cases wilds _.
+subst wilds. unfold casewild.
+unfold rl_wf. simpl.
+
+(*Need to prove that compile_size_bound is smaller with dispatch - is that true?
+  it is (length) * max (s_args) - it gets bigger
+  really, we want to ensure that it is bigger than simplified version*)
+admit.
+Admitted.
+Next Obligation.
+intros t ty tl n phd ptl Hn compile rl css is_constr types_cslist t2 Heqt2 types cslist casewild cases wilds _.
+subst wilds. unfold casewild.
+unfold compile_size'. simpl. eapply Nat.lt_le_trans. apply (dispatch_smaller n).
+(*In wilds, what is actually strictly smaller?*)
+rewrite compile_size_cons.
+apply Nat.add_le_mono_l.
+apply dispatch1_smaller.
+Defined.
+Next Obligation.
+
+
+Print dispatch1.
+
+
+Lemma dispatch_smaller n t types rhd rtl:
+  compile_size n (snd (dispatch t types rhd rtl)) <= pat_list_size_mixed n (fst rhd) + compile_size n (snd rtl).
+
+unfold dispatch1.
+
+Print dispatch1.
+Check dispatch_smaller.
+simpl.
+
+ Search compile_size.
+
+
 intros t ty tl phd ptl compile rl css is_constr types_cslist types cslist casewild cases wilds _.
 subst wilds. unfold casewild.
 rewrite dispatch_equiv.
